FiatFormal/Language/ProgressP.v
@@ -10,12 +10,11 @@ Require Import FiatFormal.Language.Progress.
 Theorem progressP
   : forall p,
     (exists t, TYPEPROG nil nil p t)
-    -> valueP p \/ (exists p', STEPP p p'). (* \/ hasChoiceP p. *)
+    -> valueP p \/ (exists p', STEPP p p') \/ hasChoiceP p.
 Proof.
-  intros.
-  induction p.
+  intros. induction p.
   Case "PLet".
-  right.
+  right. left.
   destruct H as [tp].
   inverts H.
   invert_adt_type.
@@ -26,64 +25,42 @@ Proof.
   invert_prog_type.
   rename x into t.
   pose proof (progress e).
-  destruct H. eexists. eassumption. (* TODO: ask ben why ex_spec *)
-                                (* doesn't match here *)
+  destruct H as [| []];
+
+  eauto.
+  SCase "e value".
   left; repeat constructor.
   inversion H; auto.
   unfold closedP. simpl.
-  inversion H. unfold closedX in *. assumption. (* TODO: ask ben how *)
-  (* to write Ltac to automate this *)
-  right. dest H. exists (PEXP x'). auto.
+  inversion H. unfold closedX in *. assumption.
+
+  SCase "e steps".
+  right. left. dest H. exists (PEXP x'). auto.
+
+  SCase "e hasChoice".
+  repeat right.
+  inversion H.
+
+  (* intros. *)
+  (* induction p. *)
+  (* Case "PLet". *)
+  (* right. *)
+  (* destruct H as [tp]. *)
+  (* inverts H. *)
+  (* invert_adt_type. *)
+  (* eexists. *)
+  (* eapply SP_Prog. *)
+  (* Case "PExp". *)
+  (* inverts H. *)
+  (* invert_prog_type. *)
+  (* rename x into t. *)
+  (* pose proof (progress e). *)
+  (* destruct H. eexists. eassumption. (* TODO: ask ben why ex_spec *) *)
+  (*                               (* doesn't match here *) *)
+  (* left; repeat constructor. *)
+  (* inversion H; auto. *)
+  (* unfold closedP. simpl. *)
+  (* inversion H. unfold closedX in *. assumption. (* TODO: ask ben how *) *)
+  (* (* to write Ltac to automate this *) *)
+  (* right. dest H. exists (PEXP x'). auto. *)
 Qed.
-
-(*  intros. *)
-(*  induction p; destruct H as [tx]. *)
-
-(*  Case "XVar". *)
-(*   inverts H. false. *)
-
-(*  Case "XLAM". *)
-(*   left. apply type_wfX in H. auto. *)
-
-(*  Case "XAPP". *)
-(*   inverts H. *)
-(*   destruct IHx. eauto. *)
-(*   SCase "x value". *)
-(*    right. inverts H. inverts H4. *)
-(*     inverts H1. false. *)
-(*     inverts H0. *)
-(*     exists (substTX 0 t x1). eapply ESLAMAPP. *)
-(*     inverts H0. *)
-(*   SCase "x steps". *)
-(*    right. *)
-(*     destruct H as [x']. *)
-(*     exists (XAPP x' t). *)
-(*     apply ESAPP1. auto. *)
-
-(*  Case "XLam". *)
-(*   left. apply type_wfX in H. auto. *)
-
-(*  Case "XApp". *)
-(*   right. *)
-(*   inverts H. *)
-(*   destruct IHx1; eauto. *)
-(*   SCase "x1 value". *)
-(*    destruct IHx2; eauto. *)
-(*    inverts H. *)
-
-(*    SSCase "x2 value". *)
-(*     inverts H1. *)
-(*      inverts H2. false. *)
-(*      inverts H4. *)
-(*      exists (substXX 0 x2 x0). apply ESLamApp. auto. *)
-
-(*    SSCase "x2 steps". *)
-(*     destruct H0 as [x2']. *)
-(*     exists (XApp x1 x2'). *)
-(*     apply ESApp2; auto. *)
-
-(*   SCase "x1 steps". *)
-(*    destruct H as [x1']. *)
-(*    exists (XApp x1' x2). *)
-(*    apply ESApp1; auto. *)
-(* Qed. *)
