FiatFormal/Language/SubstExistential.v
@@ -1,7 +1,9 @@
 
 Require Import FiatFormal.Language.SubstExpExp.
+Require Import FiatFormal.Language.SubstTypeExp.
 Require Import FiatFormal.Language.TyJudge.
 Require Import FiatFormal.Language.SubstTypeType.
+
 
 Theorem subst_exp_prog_ix :
   forall ke te t1 ix p t2 s,
@@ -47,6 +49,57 @@ Proof.
   eapply subst_exp_prog_ix; simpl; eauto.
 Qed.
 
+Theorem subst_type_prog_ix
+  : forall ix ke kx S te p t,
+    get ix ke = Some kx
+    -> KIND (delete ix ke) S kx
+    -> TYPEPROG ke te p t
+    -> TYPEPROG (delete ix ke) (substTE ix S te) (substTP ix S p) (substTT ix S t).
+Proof.
+  intros. gen S ix kx.
+  induction H1; intros.
+  Case "PLet".
+  simpl. invert H; intros; subst.
+  assert
+    (Hcomp : substTT (0 + ix) S (substTT 0 τr t2)
+             = (substTT 0 (substTT (0 + ix) S τr)
+                        (substTT (1 + 0 + ix) (liftTT 0 S) t2))).
+  apply substTT_substTT with (n:=0) (m:=ix).
+  simpl in Hcomp.
+  rewrite Hcomp.
+  apply TYLet.
+  SCase "ADT".
+  apply TYADT.
+  eapply subst_type_type_ix.
+  eassumption.
+  assumption.
+  assumption.
+  assert (Hcomp' : substTT (0 + ix) S (substTT 0 τr τ)
+                   = (substTT 0 (substTT (0 + ix) S τr)
+                              (substTT (1 + 0 + ix) (liftTT 0 S) τ))).
+  apply substTT_substTT with (n:=0) (m:=ix).
+  simpl in Hcomp'.
+  rewrite <- Hcomp'.
+  eapply subst_type_exp_ix.
+  eassumption.
+  assumption.
+  assumption.
+  SCase "PROG".
+  rewrite delete_rewind in *.
+  rewrite liftTE_substTE with (n:=0) (n':=ix).
+  eapply IHTYPEPROG.
+  simpl.
+  eassumption.
+  simpl.
+  eapply liftTT_weaken.
+  assumption.
+  Case "PExp".
+  apply TYExp.
+  eapply subst_type_exp_ix.
+  eassumption.
+  assumption.
+  assumption.
+Qed.
 
 Theorem subst_type_prog
   : forall ke te X S p t,
@@ -54,166 +107,31 @@ Theorem subst_type_prog
     -> KIND ke S KStar
     -> TYPEPROG ke (substTE 0 S te) (substTP 0 S p) (substTT 0 S t).
 Proof.
-Admitted.
+  intros.
+  assert (ke = delete 0 (ke :> X)). auto.
+  rewrite H1.
+  eapply subst_type_prog_ix; simpl; eauto.
+  destruct X; assumption.
+Qed.
 
+(* Main lemma supporting preservation *)
 Theorem subst_ADT_prog :
-  forall X r t1 t2 x p,
+  forall X r kr t1 t2 x p,
     TYPEPROG (nil :> X) (nil :> t1) p t2
+    -> KIND nil r kr
     -> TYPE nil nil x (substTT 0 r t1)
     -> TYPEPROG nil nil (substXP 0 x (substTP 0 r p)) (substTT 0 r t2).
 Proof.
-Admitted.
-
-(* ------------------------------------------------------------ *)
-
-
-(* Substitution lemma for substituting ADT contents into ADTs.
-   This is unnecessary if we further restrict ADTs such that method bodies may
-   not contain references to previously-bound ADTs.
-
-   Note that substituting a type into an expression can instantiate
-   type variables, so we also need to perform the substitution
-   to the result type.
- *)
-
-(* Theorem subst_exist_exp *)
-(*   : forall ke te t1 kr k2 tr x1 t2 x, *)
-(*     KIND ke tr kr *)
-(*     -> KIND ke t2 k2 *)
-(*     -> TYPE ke te x1 (substTT 0 tr t1) *)
-(*     -> TYPE (ke :> kr) (te :> t1) x t2 *)
-(*     -> TYPE ke te (substTX 0 tr (substXX 0 x1 x)) t2. *)
-(* Proof. *)
-(*   intros. gen ke te t1 kr k2 tr x1 t2. *)
-(*   induction x; intros. *)
-(*   Case "XVar". *)
-(*   simpl. *)
-(*   lift_cases. *)
-(*   inverts H2. simpl in *. *)
-(*   norm_inverts_option. *)
-(* Admitted. *)
-
-
-(* Substitution lemma for substituting ADT contents into ADTs.
-   This is unnecessary if we further restrict ADTs such that method bodies may
-   not contain references to previously-bound ADTs.
-
-   Note that substituting a type into an expression can instantiate
-   type variables, so we also need to perform the substitution
-   to the result type.
- *)
-
-(* Not clear that this particular statement is what I want *)
-(* Theorem subst_exist_adt *)
-(*   : forall ke te t1 kr tr x1 t2 ad, *)
-(*     KIND ke tr kr (* well-kinded rep type *) *)
-(*     -> TYPE ke te x1 (substTT 0 tr t1) (* existential well-typed *) *)
-(*     -> TYPEADT (ke :> kr) (te :> t1) ad t2 *)
-(*     -> TYPEADT ke te (substTADT 0 tr (substXADT 0 x1 ad)) t2. *)
-(* Proof. *)
-(*   intros. gen ke te t1 kr tr x1 t2. *)
-(*   induction ad; intros. *)
-(* Admitted. *)
-
-
-(* Main substitution lemma for substituting ADT contents into program.
-   If an ADT's methods implement their abstract interfaces,
-   substituting method bodies and representation types in program
-   preserves type.
-
-   Note that substituting a type into an expression can instantiate
-   type variables, so we also need to perform the substitution
-   to the result type.
- *)
-
-(* Theorem subst_exist_prog *)
-(*   : forall ke te t1 kr tr x1 t2 p, *)
-(*     KIND ke tr kr (* well-kinded rep type *) *)
-(*     -> TYPE ke te x1 (substTT 0 tr t1) (* existential well-typed *) *)
-(*     -> TYPEPROG (ke :> kr) (te :> t1) p t2 (* program well-typed with extended contexts *) *)
-(*     -> TYPEPROG ke te (substTP 0 tr (substXP 0 x1 p)) t2. *)
-(* Proof. *)
-(*   intros. *)
-(*   gen ke te t1 kr tr x1 t2. *)
-(*   induction p; intros. *)
-(*   Case "PLet". *)
-(*   simpl; destruct a; simpl. *)
-(*   eapply TYLet. *)
-(* Abort. *)
-
-(* Theorem subst_exist_prog_ix *)
-(*   : forall ix ix' ke te k t tr t2 x1 p, *)
-(*     get ix ke = Some k *)
-(*     -> get ix' te = Some t *)
-(*     -> KIND (delete ix ke) tr k *)
-(*     -> TYPEPROG ke te p t2 *)
-(*     (* NOTE: the liftTT-ing for taur below shouldn't be necessary, just not sure where the simple condition on rep types should ultimately be stated *) *)
-(*     -> TYPE (delete ix ke) (delete ix' te) x1 (substTT 0 tr t) *)
-(*     -> TYPEPROG (delete ix ke) (delete ix' te) (substTP 0 tr (substXP 0 x1 p)) t2. *)
-(* Proof. *)
-(* Abort. *)
-  (* intros. *)
-  (* gen ix ix' ke te k. (* TODO: ask why gen fails with all idents in a single invocation *) *)
-  (* gen t tr t2 x1. *)
-  (* induction p; intros. *)
-  (* Case "PLet". *)
-  (* simpl; destruct a; simpl. *)
-  (* eapply TYLet. *)
-  (* SCase "ADT". *)
-
-(* Theorem subst_type_exp_ix *)
-(*   : forall ix ke te x1 t1 t2 k2, *)
-(*     get ix ke = Some k2 *)
-(*     -> TYPE ke  te x1 t1 *)
-(*     -> KIND (delete ix ke)  t2 k2 *)
-(*     -> TYPE (delete ix ke)     (substTE ix t2 te) *)
-(*            (substTX ix t2 x1) (substTT ix t2 t1). *)
-(* Proof. *)
-
-(*  intros. gen ix ke te t1 t2 k2. *)
-(*  induction x1; intros; simpl; inverts H0; eauto. *)
-
-(*  Case "XVar". *)
-(*   apply TYVar. *)
-(*   unfold substTE. eapply get_map. auto. *)
-(*   eapply subst_type_type_ix; eauto. *)
-
-(*  Case "XLAM". *)
-(*   simpl. apply TYLAM. *)
-(*   rewrite delete_rewind. *)
-(*   rewrite (liftTE_substTE 0 ix). *)
-(*   eapply IHx1; eauto. *)
-(*    apply liftTT_weaken. auto. *)
-
-(*  Case "XAPP". *)
-(*   rewrite (substTT_substTT 0 ix). *)
-(*   apply TYAPP. *)
-(*    simpl. eapply (IHx1 ix) in H6; eauto. *)
-(*    simpl. eapply subst_type_type_ix; eauto. *)
-
-(*  Case "XLam". *)
-(*   simpl. apply TYLam. *)
-(*   eapply subst_type_type_ix; eauto. *)
-(*   unfold substTE. rewrite map_rewind. *)
-(*   assert ( map (substTT ix t2) (te :> t) *)
-(*          = substTE ix t2 (te :> t)). auto. *)
-(*   rewrite H0. *)
-(*    eapply IHx1; eauto. *)
-
-(*  Case "XApp". *)
-(*   eapply TYApp. *)
-(*    eapply IHx1_1 in H6; eauto. *)
-(*    eapply IHx1_2 in H8; eauto. *)
-(* Qed. *)
-
-(* Theorem subst_type_value *)
-(*  :  forall ke te x1 t1 t2 k2 *)
-(*  ,  TYPE (ke :> k2) te x1 t1 *)
-(*  -> KIND ke  t2 k2 *)
-(*  -> TYPE ke                (substTE 0 t2 te) *)
-(*          (substTX 0 t2 x1) (substTT 0 t2 t1). *)
-(* Proof. *)
-(*  intros. *)
-(*  assert (ke = delete 0 (ke :> k2)). auto. rewrite H1. *)
-(*  eapply subst_type_exp_ix; simpl; eauto. *)
-(* Qed. *)
+  intros X r kr t1 t2 x p HP HK HT.
+  pose proof (subst_type_prog) as STP.
+  specialize (STP _ _ _ r _ _ HP).
+  pose proof
+       (subst_exp_prog nil nil (substTT 0 r t1) (substTP 0 r p) (substTT 0 r t2))
+    as ESL.
+  simpl in *.
+  destruct kr.
+  specialize (STP HK).
+  specialize (ESL x STP).
+  specialize (ESL HT).
+  assumption.
+Qed.
